Finished up through DINO correctness proof; cleaning up now

semantics/algorithms.v
@@ -23,36 +23,36 @@ WAR_Skip: forall(N W R: warvars),
              (x: smallvar) (e: exp),
              isNV x -> (*checking x is nonvolatile*)
              (rd e Re) -> (*extra premise checking that Re is the list of values read when e is evaluated*)
-             not(memberwv_wv (inl x) (R ++ Re)) 
+             not(In (inl x) (R ++ Re)) 
              -> WAR_ins N W R (asgn_sv x e) ((inl x)::W) (R ++ Re)
 | WAR_Checkpointed: forall(N W R Re: warvars)
              (x: smallvar) (e: exp),
              (rd e Re) -> (*extra premise checking that Re is the list of values read when e is evaluated*)
              isNV x -> (*checking x is nonvolatile*)
-             memberwv_wv (inl x) (R ++ Re) ->
-             not(memberwv_wv (inl x) W) ->
-             (memberwv_wv (inl x) N ) ->
+             In (inl x) (R ++ Re) ->
+             not(In (inl x) W) ->
+             (In (inl x) N ) ->
              WAR_ins N W R (asgn_sv x e) ((inl x)::W) (R ++ Re)
 | WAR_WT: forall(N W R Re: warvars)
              (x: smallvar) (e: exp),
              (rd e Re) -> (*extra premise checking that Re is the list of values read when e is evaluated*)
-             memberwv_wv (inl x) (R ++ Re) ->
-             (memberwv_wv (inl x) W) ->
+             In (inl x) (R ++ Re) ->
+             (In (inl x) W) ->
              WAR_ins N W R (asgn_sv x e) W (R ++ Re)
 | WAR_NoRd_Arr: forall(N W R Re Rindex: warvars)
                  (a: array) (e index: exp)
                  (e: exp),
     (rd e Re) -> (*extra premise checking that Re is the list of values read when e is evaluated*)
     (rd index Rindex) -> (*extra premise checking that Rindex is the list of values read when index is evaluated*)
-    not(memberwv_wv (inr a) (R ++ Re ++ Rindex)) ->
+    not(In (inr a) (R ++ Re ++ Rindex)) ->
     WAR_ins N W R (asgn_arr a index e) ((inr a)::W) (R ++ Re ++ Rindex) (*written set is modified but
                                                                         don't need to check if a is NV cuz all arrays are*)
 | WAR_Checkpointed_Arr: forall(N W R Re Rindex: warvars)
                  (a: array) (e index: exp),
     (rd e Re) -> (*extra premise checking that Re is the list of values read when e is evaluated*)
     (rd index Rindex) -> (*extra premise checking that Rindex is the list of values read when index is evaluated*)
-    (memberwv_wv (inr a) (R ++ Re ++ Rindex)) ->
-    (memberwv_wv (inr a) N) ->
+    (In (inr a) (R ++ Re ++ Rindex)) ->
+    (In (inr a) N) ->
     WAR_ins N W R (asgn_arr a index e) ((inr a)::W) (R ++ Re ++ Rindex)
 .
 
@@ -62,7 +62,7 @@ Inductive WARok: warvars -> warvars -> warvars -> command -> Prop:=
  | WAR_CP: forall(w N W R: warvars) (c: command),
        WARok w nil nil c ->
        WARok N W R ((incheckpoint w);;c)
- | WAR_Seq: forall(N W W' R R': warvars)
+ | WAR_Seq: forall(N W R W' R': warvars)
              (l: instruction) (c: command),
              WAR_ins N W R l W' R' ->
              WARok N W' R' c ->
@@ -88,30 +88,32 @@ Inductive DINO_ins: warvars -> warvars -> warvars -> instruction
                   (x: smallvar) (e: exp),
              (rd e Re) -> (*extra premise checking that Re is the list of values read when e is evaluated*)
              isNV x -> (*checking x is nonvolatile*)
-             not(memberwv_wv (inl x) (R ++ Re))
+             not(In (inl x) (R ++ Re))
              -> DINO_ins N W R (asgn_sv x e) N ((inl x)::W) (R ++ Re)
 | D_WAR_CP_Asgn: forall(N W R Re: warvars) (x: smallvar) (e: exp), (*Changed name to avoid duplication w D_WAR_CP below*)
              (rd e Re) -> (*extra premise checking that Re is the list of values read when e is evaluated*)
              isNV x -> (*checking x is nonvolatile*)
-             memberwv_wv (inl x) (R ++ Re) ->
-             not(memberwv_wv (inl x) W) ->
+             In (inl x) (R ++ Re) ->
+             not(In (inl x) W) ->
              DINO_ins N W R (asgn_sv x e)
                   ((inl x)::N) ((inl x)::W) (R ++ Re)
 | D_WAR_WtDom: forall(N W R Re: warvars) 
              (x: smallvar) (e: exp),
              (rd e Re) -> (*extra premise checking that Re is the list of values read when e is evaluated*)
-             memberwv_wv (inl x) (R ++ Re) ->
-             (memberwv_wv (inl x) W) ->
+             In (inl x) (R ++ Re) ->
+             (In (inl x) W) ->
              DINO_ins N W R (asgn_sv x e) N W (R ++ Re)
 | D_WAR_Wt_Arr: forall(N W R Re Rindex: warvars)
                  (a: array) (e index: exp),
     (rd e Re) -> (*extra premise checking that Re is the list of values read when e is evaluated*)
     (rd index Rindex) -> (*extra premise checking that Rindex is the list of values read when index is evaluated*)
-    not(memberwv_wv (inr a) (R ++ Re ++ Rindex)) ->
+    not(In (inr a) (R ++ Re ++ Rindex)) ->
     DINO_ins N W R (asgn_arr a index e) N ((inr a)::W) (R ++ Re ++ Rindex)
 | D_WAR_CP_Arr: forall(N W R Re Rindex: warvars)
                  (a: array) (e index: exp), 
-                 memberwv_wv (inr a) (R ++ Re ++ Rindex) ->
+    (rd e Re) -> (*extra premise checking that Re is the list of values read when e is evaluated*)
+    (rd index Rindex) -> (*extra premise checking that Rindex is the list of values read when index is evaluated*)
+                 In (inr a) (R ++ Re ++ Rindex) ->
                  DINO_ins N W R (asgn_arr a index e)
              ((inr a):: N) ((inr a)::W) (R ++ Re ++ Rindex)
 .
@@ -121,7 +123,7 @@ Inductive DINO: warvars -> warvars -> warvars -> command
   D_WAR_Instr: forall(N N' W R W' R': warvars) (l: instruction),
     DINO_ins N W R l N' W' R' ->
     DINO N W R l l N'
-| D_WAR_Seq: forall(N N' N'' W W' R R': warvars)
+| D_WAR_Seq: forall(N N' N'' W R W' R': warvars)
               (l: instruction) (c c': command),
     DINO_ins N W R l N' W' R' ->
     DINO N' W' R' c c' N''  ->
