semantics/proofs.v
@@ -3,11 +3,11 @@ From Coq Require Import Bool.Bool Init.Nat Arith.Arith Arith.EqNat
      Init.Datatypes Lists.List Strings.String Program.
 Require Export Coq.Strings.String.
 From mathcomp Require Import ssreflect ssrfun ssrbool eqtype.
+From TLC Require Import LibTactics.
 Import ListNotations.
 From Semantics Require Export algorithms.
 
 Open Scope list_scope.
-Check incl_tl.
 (*Lemma consRight: forall(A: Type) (L1 L2: list A) (a: A), incl L1 L2 -> incl L*)
 
 Lemma onePointone: forall(N N' W W' R R': warvars) (l: instruction),
@@ -25,9 +25,45 @@ Proof. intros. induction H; try(apply onePointone in H); try apply (incl_refl N)
 
 Lemma Two: forall(N N' W W' R R' N1: warvars) (l: instruction),
     DINO_ins N W R l N' W' R' -> incl N' N1 -> WAR_ins N1 W R l W' R'.
-  intros. induction H. 
-  - constructor.
-  - constructor; assumption.
-  - apply WAR_NoRd; assumption. (*have to write this case out by hand or coq applies the wrong constructor*)
-  - apply WAR_Checkpointed; (try assumption). apply H0.
+  intros. induction H; try (constructor; assumption || (apply War_noRd; assumption));
+            (apply WAR_Checkpointed || apply WAR_Checkpointed_Arr);
+            (repeat assumption); apply H0; unfold In; left; reflexivity.
+Qed.
+
+Lemma incl_app_l: forall(A: Type) (L1 L2 L3: list A),
+    incl (L1 ++ L2) L3 -> incl L1 L3.
+Proof. intros. apply (incl_tran
+                        (incl_appl L2 (incl_refl L1))
+                        H).
+Qed.
+
+Lemma incl_app_r: forall(A: Type) (L1 L2 L3: list A),
+    incl (L1 ++ L2) L3 -> incl L2 L3.
+Proof. intros. apply (incl_tran
+                        (incl_appr L1 (incl_refl L2))
+                        H).
+Qed.
+
+
+Theorem DINO_WAR_correct: forall(N W R N': warvars) (c c': command),
+    DINO N W R c c' N' -> (forall(N1: warvars), incl N' N1 -> WARok N1 W R c').
+  intros N W R c c' N' H. induction H; intros N0 Hincl.
+
+  - eapply WAR_I. applys Two H Hincl.
+  - eapply WAR_Seq. applys Two H. apply onePointtwo in H0. eauto using incl_tran.
+  (* try (eapply WAR_I || eapply WAR_Seq);
+      eapply (Two _ _ _ _ _ _ _ _ H Hincl).
+  - intros N0 Hincl. try (eapply WAR_I || eapply WAR_Seq).
+      eapply (Two _ _ _ _ _ _ _ _ H Hincl).
+  - try (intros; (eapply WAR_I || eapply WAR_Seq); eapply Two in H; apply H); try (repeat assumption).
+- intros.
+  - intros. eapply WAR_Seq. eapply Two in H. apply H.
+    apply onePointtwo in H0. apply (incl_tran H0 H1).*)
+    apply (IHDINO N0 Hincl).
+  - eapply WAR_If; (try eassumption);
+      ((apply IHDINO1; apply incl_app_l in Hincl)
+       || (apply IHDINO2; apply incl_app_r in Hincl)); assumption.
+  - intros. apply WAR_CP. apply IHDINO. apply (incl_refl N').
+  Qed.
+  (*make ltac for first two bullets*)
 Close Scope list_scope.
